enhancing proofs performance through auxiliary algebraic laws
git-svn-id: orca@286

WP1-Programming-Languages-Semantics/WP11-C-semantics/src/IMP-Lenses/hoare/algebraic_laws_abrupt_aux.thy
@@ -1,423 +1,134 @@
 
-section "Algebraic laws for abrupt designs"
-theory algebraic_laws_abrupt
-imports "../theories/utp_abrupt_designs_aux"
+section "Auxiliary algebraic laws for abrupt designs"
+theory algebraic_laws_abrupt_aux
+imports "../theories/utp_abrupt_designs"
 
 begin
-named_theorems symbolic_exec_cp
 
-subsection"Throw"
+subsection {*Abrupt semantics behavior*}
 
-lemma throw_left_zero[simp]: 
-  "(THROW\<^sub>A\<^sub>B\<^sub>R ;; Simpl\<^sub>A\<^sub>B\<^sub>R (P)) = THROW\<^sub>A\<^sub>B\<^sub>R" 
-  by rel_auto 
-
-lemma throw_right_zero_skip[simp]: 
-  "(SKIP\<^sub>A\<^sub>B\<^sub>R ;; THROW\<^sub>A\<^sub>B\<^sub>R) = THROW\<^sub>A\<^sub>B\<^sub>R" 
-  by rel_auto 
-
-lemma throw_idem [simp]: 
-  "(THROW\<^sub>A\<^sub>B\<^sub>R ;; THROW\<^sub>A\<^sub>B\<^sub>R) = THROW\<^sub>A\<^sub>B\<^sub>R" 
-  by rel_auto
-
-subsection"Skip"
-
-text{*In this section we introduce the algebraic laws of programming related to the SKIP
-      statement.*}
-
-lemma skip_c_idem [simp]:
-  "(SKIP\<^sub>A\<^sub>B\<^sub>R ;; SKIP\<^sub>A\<^sub>B\<^sub>R) = SKIP\<^sub>A\<^sub>B\<^sub>R"
-  by rel_auto
-
-lemma skip_c_left_unit[simp]: 
-  "(SKIP\<^sub>A\<^sub>B\<^sub>R ;;  Simpl\<^sub>A\<^sub>B\<^sub>R (P)) =  Simpl\<^sub>A\<^sub>B\<^sub>R (P)"
-  by rel_auto 
-
-lemma skip_c_right_unit[simp]: 
-  "(Simpl\<^sub>A\<^sub>B\<^sub>R (P)  ;;  SKIP\<^sub>A\<^sub>B\<^sub>R) =  Simpl\<^sub>A\<^sub>B\<^sub>R (P)"  
-  by rel_auto (metis option.collapse) 
-
-lemma skip_c_lift_alpha_eq:
-  "\<lceil>II\<rceil>\<^sub>A\<^sub>B\<^sub>R = ($\<Sigma>\<^sub>A\<^sub>B\<^sub>R\<acute> =\<^sub>u $\<Sigma>\<^sub>A\<^sub>B\<^sub>R)"
-  by rel_auto
-
-lemma skip_c_alpha_eq:
-  "SKIP\<^sub>A\<^sub>B\<^sub>R = Simpl\<^sub>A\<^sub>B\<^sub>R (\<not>$abrupt\<acute> \<and> $abrupt_aux\<acute> =\<^sub>u \<guillemotleft>None\<guillemotright> \<and> ($\<Sigma>\<^sub>A\<^sub>B\<^sub>R\<acute> =\<^sub>u $\<Sigma>\<^sub>A\<^sub>B\<^sub>R))"
-  by (simp add: skip_c_lift_alpha_eq skip_abr_def)
-
-lemma pre_skip_c_post: 
-  "(Simpl\<^sub>A\<^sub>B\<^sub>R \<lceil>b\<rceil>\<^sub>A\<^sub>B\<^sub>R\<^sub>< \<and> SKIP\<^sub>A\<^sub>B\<^sub>R) = (SKIP\<^sub>A\<^sub>B\<^sub>R \<and> Simpl\<^sub>A\<^sub>B\<^sub>R \<lceil>b\<rceil>\<^sub>A\<^sub>B\<^sub>R\<^sub>>)"
-  by rel_auto 
-
-lemma skip_c_var:
-  fixes x :: "(bool,  ('a, 'b) cpa) uvar"
-  shows "(Simpl\<^sub>A\<^sub>B\<^sub>R $x \<and> SKIP\<^sub>A\<^sub>B\<^sub>R) = (SKIP\<^sub>A\<^sub>B\<^sub>R \<and> Simpl\<^sub>A\<^sub>B\<^sub>R $x\<acute>)"
-  by rel_auto
-
-lemma assigns_c_id [simp]: "\<langle>id\<rangle>\<^sub>A\<^sub>B\<^sub>R = SKIP\<^sub>A\<^sub>B\<^sub>R"
+lemma Simpl_abr_idem[simp]: "Simpl\<^sub>A\<^sub>B\<^sub>R(Simpl\<^sub>A\<^sub>B\<^sub>R(P)) = Simpl\<^sub>A\<^sub>B\<^sub>R(P)"
   by (rel_auto)
 
-lemma assign_c_alt_def [symbolic_exec_cp]: 
-  "\<langle>\<sigma>\<rangle>\<^sub>A\<^sub>B\<^sub>R = Simpl\<^sub>A\<^sub>B\<^sub>R (\<not>$abrupt\<acute> \<and> $abrupt_aux\<acute> =\<^sub>u \<guillemotleft>None\<guillemotright> \<and> \<lceil>\<lceil>\<sigma>\<rceil>\<^sub>s \<dagger> II\<rceil>\<^sub>A\<^sub>B\<^sub>R)"
-  by rel_auto
+lemma Simpl_abr_Idempotent: "Idempotent Simpl\<^sub>A\<^sub>B\<^sub>R"
+  by (simp add: Idempotent_def Simpl_abr_idem)
 
-subsection {*Assignment Laws*}
-text{*In this section we introduce the algebraic laws of programming related to the assignment
-      statement.*}
+lemma Simpl_abr_mono: "P \<sqsubseteq> Q \<Longrightarrow> Simpl\<^sub>A\<^sub>B\<^sub>R(P) \<sqsubseteq> Simpl\<^sub>A\<^sub>B\<^sub>R(Q)"
+  by (rel_auto)
 
-lemma usubst_c_cancel [usubst,symbolic_exec_cp]: 
-  assumes 1:"weak_lens v" 
-  shows "($v)\<lbrakk>\<lceil>expr\<rceil>\<^sub>A\<^sub>B\<^sub>R\<^sub></$v\<rbrakk>= \<lceil>expr\<rceil>\<^sub>A\<^sub>B\<^sub>R\<^sub><"
-  using 1
-  by  rel_auto
+lemma Simpl_abr_Monotonic: "Monotonic Simpl\<^sub>A\<^sub>B\<^sub>R"
+  by (simp add: Monotonic_def Simpl_abr_mono)
 
-lemma usubst_c_lift_cancel[usubst,symbolic_exec_cp]: 
-  assumes 1:"weak_lens v" 
-  shows "\<lceil>($v)\<lbrakk>\<lceil>expr\<rceil>\<^sub></$v\<rbrakk>\<rceil>\<^sub>A\<^sub>B\<^sub>R= \<lceil>expr\<rceil>\<^sub>A\<^sub>B\<^sub>R\<^sub><"
-  using 1
-  by  rel_auto
+lemma Simpl_abr_condr: "Simpl\<^sub>A\<^sub>B\<^sub>R(P \<triangleleft> b \<triangleright> Q) = (Simpl\<^sub>A\<^sub>B\<^sub>R(P) \<triangleleft> b \<triangleright> Simpl\<^sub>A\<^sub>B\<^sub>R(Q))"
+  by (rel_auto)
 
-lemma assigns_c_comp: "(\<langle>f\<rangle>\<^sub>A\<^sub>B\<^sub>R ;; \<langle>g\<rangle>\<^sub>A\<^sub>B\<^sub>R) = \<langle>g \<circ> f\<rangle>\<^sub>A\<^sub>B\<^sub>R"
-  by rel_auto 
+lemma Simpl_abr_if_abr: 
+  "Simpl\<^sub>A\<^sub>B\<^sub>R(bif b then P else Q eif) = 
+   (bif b then Simpl\<^sub>A\<^sub>B\<^sub>R(P) else Simpl\<^sub>A\<^sub>B\<^sub>R(Q) eif)"
+  by (rel_auto)
 
-lemma assign_test[symbolic_exec_cp]:
-  assumes 1:"mwb_lens x" 
-  shows     "(x \<Midarrow> \<guillemotleft>u\<guillemotright> ;; x \<Midarrow> \<guillemotleft>v\<guillemotright>) = (x \<Midarrow> \<guillemotleft>v\<guillemotright>)"
-  using 1   
-  by (simp add: assigns_c_comp subst_upd_comp subst_lit usubst_upd_idem)
+lemma Simpl_abr_skip_abr[simp]: "Simpl\<^sub>A\<^sub>B\<^sub>R(SKIP\<^sub>A\<^sub>B\<^sub>R) = (SKIP\<^sub>A\<^sub>B\<^sub>R)"
+  by (rel_auto)
+                    
+lemma Simpl_abr_throw_abr[simp]: "Simpl\<^sub>A\<^sub>B\<^sub>R(THROW\<^sub>A\<^sub>B\<^sub>R) = (THROW\<^sub>A\<^sub>B\<^sub>R)"
+  by (rel_auto)
 
-lemma assign_c_left_comp: 
-  "(\<langle>\<sigma>\<rangle>\<^sub>A\<^sub>B\<^sub>R ;; Simpl\<^sub>A\<^sub>B\<^sub>R(\<lceil>P\<rceil>\<^sub>A\<^sub>B\<^sub>R \<turnstile> \<lceil>Q\<rceil>\<^sub>A\<^sub>B\<^sub>R)) = Simpl\<^sub>A\<^sub>B\<^sub>R(\<lceil>\<lceil>\<sigma>\<rceil>\<^sub>s \<dagger> P\<rceil>\<^sub>A\<^sub>B\<^sub>R \<turnstile> \<lceil>\<lceil>\<sigma>\<rceil>\<^sub>s \<dagger> Q\<rceil>\<^sub>A\<^sub>B\<^sub>R)"
-  by rel_auto
+lemma Simpl_abr_assign_abr[simp]: "Simpl\<^sub>A\<^sub>B\<^sub>R(\<langle>\<sigma>\<rangle>\<^sub>A\<^sub>B\<^sub>R) = (\<langle>\<sigma>\<rangle>\<^sub>A\<^sub>B\<^sub>R)"
+  by (rel_auto)
 
-lemma assign_c_left_comp_subst[symbolic_exec_cp]: 
-  "(x \<Midarrow> u ;; Simpl\<^sub>A\<^sub>B\<^sub>R(\<lceil>P\<rceil>\<^sub>A\<^sub>B\<^sub>R \<turnstile> \<lceil>Q\<rceil>\<^sub>A\<^sub>B\<^sub>R)) = Simpl\<^sub>A\<^sub>B\<^sub>R(\<lceil>P\<lbrakk>\<lceil>u\<rceil>\<^sub></$x\<rbrakk>\<rceil>\<^sub>A\<^sub>B\<^sub>R \<turnstile> \<lceil>Q\<lbrakk>\<lceil>u\<rceil>\<^sub></$x\<rbrakk>\<rceil>\<^sub>A\<^sub>B\<^sub>R)" 
-  by rel_auto
+lemma Simpl_abr_form: "Simpl\<^sub>A\<^sub>B\<^sub>R(P) = ((\<not> (\<not>$abrupt \<and> ($abrupt_aux =\<^sub>u \<guillemotleft>None\<guillemotright>)) \<and> II) \<or> 
+                              (\<not>$abrupt \<and> $abrupt_aux =\<^sub>u \<guillemotleft>None\<guillemotright> \<and> (\<lceil>true\<rceil>\<^sub>A\<^sub>B\<^sub>R \<turnstile> (P))))"
+  by (rel_auto) 
 
-lemma assign_c_twice[symbolic_exec_cp]: 
-  assumes "mwb_lens x" and  "x \<sharp> f" 
-  shows "(x \<Midarrow> e ;; x \<Midarrow> f) = (x \<Midarrow> f)" 
+lemma abrupt_Simpl_abr:
+  "(\<not> (\<not>$abrupt \<and> ($abrupt_aux =\<^sub>u \<guillemotleft>None\<guillemotright>)) \<and> Simpl\<^sub>A\<^sub>B\<^sub>R(P)) = 
+   (II \<and> \<not> (\<not>$abrupt\<acute> \<and> ($abrupt_aux\<acute> =\<^sub>u \<guillemotleft>None\<guillemotright>)))"
+  by (rel_auto)
+
+lemma nabrupt_Simpl_abr:
+  "(\<not>$abrupt \<and> $abrupt_aux =\<^sub>u \<guillemotleft>None\<guillemotright> \<and> Simpl\<^sub>A\<^sub>B\<^sub>R(P)) = 
+   (\<not>$abrupt \<and> $abrupt_aux =\<^sub>u \<guillemotleft>None\<guillemotright> \<and> (\<lceil>true\<rceil>\<^sub>A\<^sub>B\<^sub>R \<turnstile> (P)))"
+  by (rel_auto)
+
+lemma Simpl_abr_semir_form:
+  "(Simpl\<^sub>A\<^sub>B\<^sub>R(P) ;; Simpl\<^sub>A\<^sub>B\<^sub>R(Q)) = Simpl\<^sub>A\<^sub>B\<^sub>R((\<lceil>true\<rceil>\<^sub>A\<^sub>B\<^sub>R \<turnstile> (P)) ;; Simpl\<^sub>A\<^sub>B\<^sub>R(Q))"
+  by (rel_simp) blast 
+
+lemma Simpl_abr_semir_closure:
+  assumes "P is Simpl\<^sub>A\<^sub>B\<^sub>R" "Q is Simpl\<^sub>A\<^sub>B\<^sub>R"
+  shows "(P ;; Q) is Simpl\<^sub>A\<^sub>B\<^sub>R"
   using assms
-  by (simp add: assigns_c_comp usubst)
-   
-lemma assign_c_commute:
-  assumes "x \<bowtie> y" "x \<sharp> f" "y \<sharp> e"
-  shows "(x \<Midarrow> e ;; y \<Midarrow> f) = (y \<Midarrow> f ;; x \<Midarrow> e)"
-proof -
-  have "(x :== e ;; y :== f ) = y :== f ;; x :== e"
-    using assms assign_commute by auto 
-  then show ?thesis
-    using assigns_c_comp assigns_c_def utp_urel_laws.assigns_comp
-    by metis
-qed
-  
-lemma assign_c_cond_c[symbolic_exec_cp]:
-  fixes x :: "('a, '\<alpha>) uvar"
-  shows "(x \<Midarrow> e ;; (bif b then P else Q eif)) = 
-         (bif (b\<lbrakk>e/x\<rbrakk>) then (x \<Midarrow> e ;; P)  else (x \<Midarrow> e ;; Q) eif)"
-  by rel_auto (blast)+
+  by (metis  Healthy_def Simpl_abr_semir_form Simpl_abr_idem)
 
-lemma assign_c_uop1[symbolic_exec_cp]: 
-  assumes 1: "mwb_lens v"
-  shows "(v \<Midarrow> e1 ;; v \<Midarrow> (uop F (&v))) = (v \<Midarrow> (uop F e1))"
-  by (simp add: assigns_c_comp assms subst_uop subst_upd_comp subst_var 
-                usubst_lookup_upd usubst_upd_idem)
+definition design_abr_sup :: "('a,'\<alpha>,'\<beta>) rel_cpa set \<Rightarrow> ('a,'\<alpha>,'\<beta>) rel_cpa" ("\<Sqinter>\<^sub>A\<^sub>B\<^sub>R_" [900] 900) where
+"\<Sqinter>\<^sub>A\<^sub>B\<^sub>R A = (if (A = {}) then \<top>\<^sub>A\<^sub>B\<^sub>R else \<Sqinter> A)"
 
-lemma assign_c_bop1[symbolic_exec_cp]: 
-  assumes 1: "mwb_lens v" and 2:"v \<sharp> e2"
-  shows "(v \<Midarrow> e1 ;; v \<Midarrow>(bop bp (&v) e2)) = (v \<Midarrow> (bop bp e1 e2))"
-  using 1 2  
-  by rel_auto (metis mwb_lens.put_put mwb_lens_weak weak_lens.put_get)
+lemma Simpl_abr_Continuous: "Continuous Simpl\<^sub>A\<^sub>B\<^sub>R"
+  unfolding Continuous_def SUP_def apply rel_simp
+  unfolding  SUP_def  
+  apply transfer apply auto 
+done
 
-lemma assign_c_bop2[symbolic_exec_cp]: 
-  assumes 1: "mwb_lens v" and 2:"v \<sharp> e2"
-  shows "(v \<Midarrow> e1 ;; v \<Midarrow> (bop bp e2 (&v))) = (v \<Midarrow> (bop bp e2 e1))"
-  using 1 2  
-  by rel_auto (metis mwb_lens.put_put mwb_lens_weak weak_lens.put_get)
+lemma Simpl_abr_R3_conj: "Simpl\<^sub>A\<^sub>B\<^sub>R(P \<and> Q) = (Simpl\<^sub>A\<^sub>B\<^sub>R(P) \<and> Simpl\<^sub>A\<^sub>B\<^sub>R(Q))"
+  by (rel_auto)
 
-lemma assign_c_trop1[symbolic_exec_cp]: 
-  assumes 1: "mwb_lens v" and 2:"v \<sharp> e2" and 3:"v \<sharp> e3"
-  shows "(v \<Midarrow> e1 ;; v \<Midarrow> (trop tp (&v) e2 e3)) = 
-         (v \<Midarrow> (trop tp e1 e2 e3))"
-  using 1 2 3
-  by rel_auto (metis mwb_lens.put_put mwb_lens_weak weak_lens.put_get)
+lemma Simpl_abr_disj: "Simpl\<^sub>A\<^sub>B\<^sub>R(P \<or> Q) = (Simpl\<^sub>A\<^sub>B\<^sub>R(P) \<or> Simpl\<^sub>A\<^sub>B\<^sub>R(Q))"
+  by (rel_auto)
 
-lemma assign_c_trop2[symbolic_exec_cp]: 
-  assumes 1: "mwb_lens v" and 2:"v \<sharp> e2" and 3:"v \<sharp> e3"
-  shows "(v \<Midarrow> e1 ;; v \<Midarrow> (trop tp e2 (&v) e3)) = 
-         (v \<Midarrow> (trop tp e2 e1 e3))"
-  using 1 2 3
-  by rel_auto (metis mwb_lens.put_put mwb_lens_weak weak_lens.put_get)
+lemma Simpl_abr_USUP:
+  assumes "A \<noteq> {}"
+  shows "Simpl\<^sub>A\<^sub>B\<^sub>R(\<Sqinter> i \<in> A \<bullet> P(i)) = (\<Sqinter> i \<in> A \<bullet> Simpl\<^sub>A\<^sub>B\<^sub>R(P(i)))"
+  using assms by (rel_auto)
 
-lemma assign_c_trop3[symbolic_exec_cp]: 
-  assumes 1: "mwb_lens v" and 2:"v \<sharp> e2" and 3:"v \<sharp> e3"
-  shows "(v \<Midarrow> e1 ;; v \<Midarrow> (trop tp e2 e3 (&v))) = 
-         (v \<Midarrow> (trop tp e2 e3 e1))"
-  using 1 2 3
-  by rel_auto (metis mwb_lens.put_put mwb_lens_weak weak_lens.put_get)
 
-lemma assign_c_qtop1[symbolic_exec_cp]: 
-  assumes 1: "mwb_lens v" and 2:"v \<sharp> e2" and 3:"v \<sharp> e3" and 4:"v \<sharp> e4"
-  shows "(v \<Midarrow> e1 ;; v \<Midarrow> (qtop tp (&v) e2 e3 e4)) = 
-         (v \<Midarrow> (qtop tp e1 e2 e3 e4))"
-  using 1 2 3 4
-  by rel_auto (metis mwb_lens.put_put mwb_lens_weak weak_lens.put_get)
+lemma design_abr_sup_non_empty [simp]:  
+  "A \<noteq> {} \<Longrightarrow> \<Sqinter>\<^sub>A\<^sub>B\<^sub>R A = \<Sqinter> A"
+  by (simp add: design_abr_sup_def)
 
-lemma assign_c_qtop2[symbolic_exec_cp]: 
-  assumes 1: "mwb_lens v" and 2:"v \<sharp> e2" and 3:"v \<sharp> e3" and 4:"v \<sharp> e4"
-  shows "(v \<Midarrow> e1 ;; v \<Midarrow> (qtop tp e2 (&v) e3 e4)) = 
-         (v \<Midarrow> (qtop tp e2 e1 e3 e4))"
-  using 1 2 3 4
-  by rel_auto (metis mwb_lens.put_put mwb_lens_weak weak_lens.put_get)
+subsection {*Abrupt top behavior*}
 
-lemma assign_c_qtop3[symbolic_exec_cp]: 
-  assumes 1: "mwb_lens v" and 2:"v \<sharp> e2" and 3:"v \<sharp> e3" and 4:"v \<sharp> e4"
-  shows "(v \<Midarrow> e1 ;; v \<Midarrow> (qtop tp e2 e3 (&v) e4)) = 
-         (v \<Midarrow> (qtop tp e2 e3 e1 e4))"
-  using 1 2 3 4
-  by rel_auto (metis mwb_lens.put_put mwb_lens_weak weak_lens.put_get)
+theorem design_top_abr_left_zero[simp]: 
+  "(\<top>\<^sub>A\<^sub>B\<^sub>R ;; (P \<turnstile> Q)) = \<top>\<^sub>A\<^sub>B\<^sub>R"
+  by (rel_auto)
 
-lemma assign_c_qtop4[symbolic_exec_cp]: 
-  assumes 1: "mwb_lens v" and 2:"v \<sharp> e2" and 3:"v \<sharp> e3" and 4:"v \<sharp> e4"
-  shows "(v \<Midarrow> e1 ;; v \<Midarrow> (qtop tp e2 e3 e4 (&v))) = 
-         (v \<Midarrow> (qtop tp e2 e3 e4 e1))"
-  using 1 2 3 4
-  by rel_auto (metis mwb_lens.put_put mwb_lens_weak weak_lens.put_get)
+theorem Simpl_abr_top_abr_left_zero[simp]: 
+  "(\<top>\<^sub>A\<^sub>B\<^sub>R ;; Simpl\<^sub>A\<^sub>B\<^sub>R (P)) = \<top>\<^sub>A\<^sub>B\<^sub>R"
+  by (rel_auto)
 
-lemma assign_c_cond_seqr_dist[symbolic_exec_cp]:
-  "(bif (b\<lbrakk>e/v\<rbrakk>) then (v \<Midarrow> e ;; P) else (v \<Midarrow> e ;; Q) eif) = 
-   (v \<Midarrow> e ;; bif b then P else Q eif)"
-  by (metis assign_c_cond_c) 
+lemma design_top_abr:
+  "(P \<turnstile> Q) \<sqsubseteq> \<top>\<^sub>A\<^sub>B\<^sub>R"
+  by (rel_auto)
 
-text {*In the sequel we define assignment laws proposed by Hoare*}
+lemma Simpl_abr_top_abr:
+  "Simpl\<^sub>A\<^sub>B\<^sub>R (P) \<sqsubseteq> \<top>\<^sub>A\<^sub>B\<^sub>R"
+  by (rel_auto)
 
-lemma assign_c_vwb_skip_c:
-  assumes 1: "vwb_lens v"
-  shows "(v \<Midarrow> &v) = SKIP\<^sub>A\<^sub>B\<^sub>R"
-  by (simp add: assms  usubst_upd_var_id)
+lemma design_abr_sup_empty [simp]: 
+  "\<Sqinter>\<^sub>A\<^sub>B\<^sub>R {} = \<top>\<^sub>A\<^sub>B\<^sub>R"
+  by (simp add: design_abr_sup_def)
 
-lemma assign_c_simultaneous:
-  assumes  1: "vwb_lens var2"
-  and      2: "var1 \<bowtie> var2"
-  shows "var1, var2 \<Midarrow> exp, &var2 = var1 \<Midarrow> exp"
-  by (simp add: "1" "2" usubst_upd_comm usubst_upd_var_id)
+subsection {*Abrupt Bot behavior*}
 
-lemma assign_c_seq:
-  assumes  1: "vwb_lens var2"
-  shows"(var1 \<Midarrow> exp);; (var2 \<Midarrow> &var2) = (var1 \<Midarrow> exp)"
-  using 1 by rel_auto 
+abbreviation design_inf :: "('\<alpha>, '\<beta>) rel_des set \<Rightarrow> ('\<alpha>, '\<beta>) rel_des" ("\<Squnion>\<^sub>A\<^sub>B\<^sub>R_" [900] 900) where
+"\<Squnion>\<^sub>A\<^sub>B\<^sub>R A \<equiv> \<Squnion> A"
 
-lemma assign_c_cond_c_uop[symbolic_exec_cp]:
-  assumes 1: "weak_lens v"
-  shows "bif uop F exp then (v \<Midarrow> exp ;; C1) else (v \<Midarrow> exp ;; C2) eif = 
-          v \<Midarrow> exp ;; bif uop F (&v) then C1 else  C2 eif"
-proof -
-  have "uop F exp = uop F ((&v::('a, 'b) uexpr)\<lbrakk>exp/v\<rbrakk>)"
-    by (metis (no_types) assms  usubst_cancel)
-  then show ?thesis
-  by (smt assign_c_cond_seqr_dist subst_uop)  
-qed
+lemma design_bottom_abr:
+  "\<bottom>\<^sub>A\<^sub>B\<^sub>R \<sqsubseteq> (P \<turnstile> Q)"
+  by simp
 
-lemma assign_c_cond_bop1[symbolic_exec_cp]:
-  assumes 1: "weak_lens v" and 2: "v \<sharp> exp2"
-  shows "bif bop bp exp exp2 then (v \<Midarrow> exp ;; C1) else (v \<Midarrow> exp ;; C2) eif = 
-          v \<Midarrow> exp ;; bif bop bp (&v) exp2 then C1 else C2 eif"
- proof -
-  have "bop bp exp exp2 = bop bp ((&v::('a, 'b) uexpr)\<lbrakk>exp/v\<rbrakk>) exp2"
-    by (metis (no_types) assms(1)  usubst_cancel)
-  then show ?thesis
-    using assign_c_cond_seqr_dist subst_bop
-    by (metis (no_types, hide_lams) "2" id_subst pr_var_def subst_unrest)
-qed
+lemma Simpl_abr_bottom_abr:
+  "\<bottom>\<^sub>A\<^sub>B\<^sub>R \<sqsubseteq> Simpl\<^sub>A\<^sub>B\<^sub>R (P)"
+  by simp
 
-lemma assign_c_cond_bop2[symbolic_exec_cp]:
-  assumes 1: "weak_lens v" and 2: "v \<sharp> exp2"
-  shows "bif bop bp exp2 exp then (v \<Midarrow> exp ;; C1) else (v \<Midarrow> exp ;; C2) eif = 
-          v \<Midarrow> exp ;; bif bop bp  exp2 (&v) then C1 else C2 eif"
- proof -
-  have "bop bp exp2 exp  = bop bp  exp2 ((&v::('a, 'b) uexpr)\<lbrakk>exp/v\<rbrakk>)"
-    by (metis (no_types) assms(1)  usubst_cancel)
-  then show ?thesis
-    using assign_c_cond_seqr_dist subst_bop
-    by (metis (no_types, hide_lams) "2" id_subst pr_var_def subst_unrest)
-qed
+lemma Simpl_abr_UINF:
+  assumes "A \<noteq> {}"
+  shows "Simpl\<^sub>A\<^sub>B\<^sub>R(\<Squnion> i \<in> A \<bullet> P(i)) = (\<Squnion> i \<in> A \<bullet> Simpl\<^sub>A\<^sub>B\<^sub>R(P(i)))"
+  using assms by (rel_auto)
 
-lemma assign_cond_trop1[symbolic_exec_cp]:
-  assumes 1: "weak_lens v" and 2: "v \<sharp> exp2" and 3: "v \<sharp> exp3"
-  shows "bif trop bp exp exp2 exp3 then (v \<Midarrow> exp ;; C1) else (v \<Midarrow> exp ;; C2) eif = 
-         v \<Midarrow> exp ;; bif trop bp (&v) exp2 exp3 then C1 else C2 eif"
- proof -
-  have "trop bp exp exp2 exp3 = trop bp ((&v::('a, 'b) uexpr)\<lbrakk>exp/v\<rbrakk>) exp2 exp3"
-    by (metis (no_types) assms(1)  usubst_cancel)
-  then show ?thesis
-    using assign_c_cond_seqr_dist subst_trop
-    by (metis (no_types, hide_lams) "2" "3" id_subst pr_var_def subst_unrest)
-qed
-
-lemma assign_cond_trop2[symbolic_exec_cp]:
-  assumes 1: "weak_lens v" and 2: "v \<sharp> exp2" and 3: "v \<sharp> exp3"
-  shows "bif trop bp exp2 exp  exp3 then (v \<Midarrow> exp ;; C1) else (v \<Midarrow> exp ;; C2) eif = 
-         v \<Midarrow> exp ;; bif trop bp  exp2 (&v) exp3 then C1 else C2 eif"
- proof -
-  have "trop bp exp2 exp exp3 = trop bp exp2 ((&v::('a, 'b) uexpr)\<lbrakk>exp/v\<rbrakk>) exp3"
-    by (metis (no_types) assms(1)  usubst_cancel)
-  then show ?thesis
-    using assign_c_cond_seqr_dist subst_trop
-    by (metis (no_types, hide_lams) "2" "3" id_subst pr_var_def subst_unrest)
-qed
-
-lemma assign_cond_trop3[symbolic_exec_cp]:
-  assumes 1: "weak_lens v" and 2: "v \<sharp> exp2" and 3: "v \<sharp> exp3"
-  shows "bif trop bp exp2 exp3 exp then (v \<Midarrow> exp ;; C1) else (v \<Midarrow> exp ;; C2) eif = 
-         v \<Midarrow> exp ;; bif trop bp exp2 exp3 (&v)  then C1 else C2 eif"
- proof -
-  have "trop bp exp2 exp3 exp  = trop bp exp2 exp3 ((&v::('a, 'b) uexpr)\<lbrakk>exp/v\<rbrakk>)"
-    by (metis (no_types) assms(1)  usubst_cancel)
-  then show ?thesis
-    using assign_c_cond_seqr_dist subst_trop
-    by (metis (no_types, hide_lams) "2" "3" id_subst pr_var_def subst_unrest)
-qed
-
-lemma assign_cond_qtop1[symbolic_exec_cp]:
-  assumes 1: "weak_lens v" and 2: "v \<sharp> exp2" and 3: "v \<sharp> exp3" and 4: "v \<sharp> exp4"
-  shows "bif qtop bp exp exp2 exp3 exp4 then (v \<Midarrow> exp ;; C1) else (v \<Midarrow> exp ;; C2) eif = 
-         v \<Midarrow> exp ;; bif qtop bp (&v) exp2 exp3 exp4 then C1 else C2 eif"
- proof -
-  have "qtop bp exp exp2 exp3 exp4 = qtop bp ((&v::('a, 'b) uexpr)\<lbrakk>exp/v\<rbrakk>) exp2 exp3 exp4"
-    by (metis (no_types) assms(1)  usubst_cancel)
-  then show ?thesis
-    using assign_c_cond_seqr_dist subst_qtop
-    by (metis (no_types, hide_lams) "2" "3" "4" id_subst pr_var_def subst_unrest)
-qed
-
-lemma assign_c_cond_qtop2[symbolic_exec_cp]:
-  assumes 1: "weak_lens v" and 2: "v \<sharp> exp2" and 3: "v \<sharp> exp3" and 4:"v \<sharp> exp4"
-  shows "bif qtop bp exp2 exp  exp3 exp4 then (v \<Midarrow> exp ;; C1) else (v \<Midarrow> exp ;; C2) eif = 
-         v \<Midarrow> exp ;; bif qtop bp exp2 (&v) exp3 exp4 then C1 else C2 eif"
- proof -
-  have "qtop bp exp2 exp exp3 exp4 = qtop bp exp2 ((&v::('a, 'b) uexpr)\<lbrakk>exp/v\<rbrakk>) exp3 exp4"
-    by (metis (no_types) assms(1)  usubst_cancel)
-  then show ?thesis
-    using assign_c_cond_seqr_dist subst_qtop
-    by (metis (no_types, hide_lams) "2" "3" "4" id_subst pr_var_def subst_unrest)
-qed
-
-lemma assign_c_cond_qtop3[symbolic_exec_cp]:
-  assumes 1: "weak_lens v" and 2: "v \<sharp> exp2" and 3: "v \<sharp> exp3" and 4: "v \<sharp> exp4"
-  shows "bif qtop bp exp2 exp3 exp exp4 then (v \<Midarrow> exp ;; C1) else (v \<Midarrow> exp ;; C2) eif = 
-         v \<Midarrow> exp ;; bif qtop bp exp2  exp3 (&v) exp4 then C1 else C2 eif"
- proof -
-  have "qtop bp exp2 exp3 exp  exp4 = qtop bp exp2  exp3 ((&v::('a, 'b) uexpr)\<lbrakk>exp/v\<rbrakk>) exp4"
-    by (metis (no_types) assms(1)  usubst_cancel)
-  then show ?thesis
-    using assign_c_cond_seqr_dist subst_qtop
-    by (metis (no_types, hide_lams) "2" "3" "4" id_subst pr_var_def subst_unrest)
-qed
-
-lemma assign_c_cond_qtop4[symbolic_exec_cp]:
-  assumes 1: "weak_lens v" and 2: "v \<sharp> exp2" and 3: "v \<sharp> exp3" and 4: "v \<sharp> exp4"
-  shows "bif qtop bp exp2 exp3 exp4 exp then (v \<Midarrow> exp ;; C1) else (v \<Midarrow> exp ;; C2) eif = 
-         v \<Midarrow> exp ;; bif qtop bp exp2  exp3 exp4 (&v)  then C1 else C2 eif"
- proof -
-  have "qtop bp exp2 exp3 exp4 exp = qtop bp exp2 exp3 exp4 ((&v::('a, 'b) uexpr)\<lbrakk>exp/v\<rbrakk>)"
-    by (metis (no_types) assms(1)  usubst_cancel)
-  then show ?thesis
-    using assign_c_cond_seqr_dist subst_qtop
-    by (metis (no_types, hide_lams) "2" "3" "4" id_subst pr_var_def subst_unrest)
-qed
-
-lemma assign_c_cond_If [symbolic_exec_cp]:
-  "(bif bexp then (v \<Midarrow> exp1) else (v \<Midarrow> exp2) eif) = 
-   (v \<Midarrow> (trop If bexp exp1 exp2))" 
-  by rel_auto
-
-subsection {*While laws*}
-text{*In this section we introduce the algebraic laws of programming related to the while
-      statement.*}
+subsection {*Abrupt If behavior*}
 
 lemma if_mono:
   "\<lbrakk> P\<^sub>1 \<sqsubseteq> P\<^sub>2; Q\<^sub>1 \<sqsubseteq> Q\<^sub>2 \<rbrakk> \<Longrightarrow> (bif b then P\<^sub>1 else Q\<^sub>1 eif) \<sqsubseteq> (bif b then P\<^sub>2 else Q\<^sub>2 eif)"
   by rel_auto
-
-theorem while_unfold:
-  "while b do P od = (bif b then (P ;; while b do P od) else SKIP\<^sub>A\<^sub>B\<^sub>R eif)"
-proof -
-  have m:"mono (\<lambda>X. bif b then (P ;; X) else SKIP\<^sub>A\<^sub>B\<^sub>R eif)"
-    by (auto intro: monoI seqr_mono if_mono)
-  have "(while b do P od) = (\<nu> X \<bullet> bif b then (P ;; X) else SKIP\<^sub>A\<^sub>B\<^sub>R eif)"
-    by (simp add: While_def)
-  also have "... = (bif b then (P ;; (\<nu> X \<bullet> bif b then (P ;; X) else SKIP\<^sub>A\<^sub>B\<^sub>R eif)) else SKIP\<^sub>A\<^sub>B\<^sub>R eif)"
-    by (subst lfp_unfold,simp_all add:m )
-  also have "... = (bif b then (P ;; while b do P od) else SKIP\<^sub>A\<^sub>B\<^sub>R eif)"
-    by (simp add: While_def)
-  finally show ?thesis .
-qed
-
-lemma design_top_abr:
-  "Simpl\<^sub>A\<^sub>B\<^sub>R (P) \<sqsubseteq> \<top>\<^sub>A\<^sub>B\<^sub>R"
-  by (rel_auto)
-
-(*lemma while_true:
-  shows "(while true do P od) = \<top>\<^sub>A\<^sub>B\<^sub>R"
-  apply (simp add: While_def alpha)
-  apply (rule antisym)
-  apply (simp_all)
-  apply (rule conjI)
-  apply (rule lfp_lowerbound)
-  apply (simp add: C3_abr_def design_def cond_def)
-  apply rel_auto
-  apply (frule cond_mono)
-done*)
-
-lemma while_false:
-  shows "(while false do P od) = SKIP\<^sub>A\<^sub>B\<^sub>R"
-proof -
-  have "(while false do P od) = bif false then (P ;; while false do P od) else SKIP\<^sub>A\<^sub>B\<^sub>R eif" 
-    using while_unfold[of _ P] by simp
-  also have "... = SKIP\<^sub>A\<^sub>B\<^sub>R" by rel_blast
-  finally show ?thesis . 
-qed
-
-lemma while_inv_unfold:
-  "while b invr p do P od = (bif b then (P ;; while b invr p do P od) else SKIP\<^sub>A\<^sub>B\<^sub>R eif)"
-  unfolding While_inv_def using while_unfold
-  by auto
-
-theorem while_bot_unfold:
-  "while\<^sub>\<bottom> b do P od = (bif b then (P ;; while\<^sub>\<bottom> b do P od) else SKIP\<^sub>A\<^sub>B\<^sub>R eif)"
-proof -
-  have m:"mono (\<lambda>X. bif b then (P ;; X) else SKIP\<^sub>A\<^sub>B\<^sub>R eif)"
-    by (auto intro: monoI seqr_mono if_mono)
-  have "(while\<^sub>\<bottom> b do P od) = (\<mu> X \<bullet> bif b then (P ;; X) else SKIP\<^sub>A\<^sub>B\<^sub>R eif)"
-    by (simp add: While_bot_def)
-  also have "... = (bif b then (P ;; (\<mu> X \<bullet> bif b then (P ;; X) else SKIP\<^sub>A\<^sub>B\<^sub>R eif)) else SKIP\<^sub>A\<^sub>B\<^sub>R eif)"
-    by (subst gfp_unfold, simp_all add: m)
-  also have "... = (bif b then (P ;; while\<^sub>\<bottom> b do P od) else SKIP\<^sub>A\<^sub>B\<^sub>R eif)"
-    by (simp add: While_bot_def)
-  finally show ?thesis .
-qed
-
-theorem while_bot_false: "while\<^sub>\<bottom> false do P od = SKIP\<^sub>A\<^sub>B\<^sub>R"
-  by (simp add: While_bot_def mu_const alpha, rel_auto)
-
-theorem while_bot_true: "while\<^sub>\<bottom> true do P od = (\<mu> X \<bullet> Simpl\<^sub>A\<^sub>B\<^sub>R (P ;; X))"
-  by (simp add: While_bot_def alpha)
-
-subsection {*assume laws*}
-
-lemma assume_twice: "(b\<^sup>\<top>\<^sup>C ;; c\<^sup>\<top>\<^sup>C) = (b \<and> c)\<^sup>\<top>\<^sup>C"
-  by (rel_auto) 
-
-lemma assert_twice: "(b\<^sub>\<bottom>\<^sub>C ;; c\<^sub>\<bottom>\<^sub>C) = (b \<and> c)\<^sub>\<bottom>\<^sub>C" 
-  apply (simp add: rassert_abr_def C3_abr_def cond_def)
-  apply pred_simp 
-  apply auto
-  apply (rel_simp)+
-  apply blast
-  apply (rel_simp)+
-  apply (metis (full_types) option.exhaust)
-  apply (rel_blast+)
-done
-
 
 end
